%%%%%%%%%%%%%%%%%%%%%%%%%%%%%%%%%%%%%%%%%
% Short Sectioned Assignment
% LaTeX Template
% Version 1.0 (5/5/12)
%
% This template has been downloaded from:
% http://www.LaTeXTemplates.com
%
% Original author:
% Frits Wenneker (http://www.howtotex.com)
%
% License:
% CC BY-NC-SA 3.0 (http://creativecommons.org/licenses/by-nc-sa/3.0/)
%
%%%%%%%%%%%%%%%%%%%%%%%%%%%%%%%%%%%%%%%%%

%----------------------------------------------------------------------------------------
%	PACKAGES AND OTHER DOCUMENT CONFIGURATIONS
%----------------------------------------------------------------------------------------

\documentclass[fontsize=11pt]{scrartcl} % 11pt font size

\usepackage[T1]{fontenc} % Use 8-bit encoding that has 256 glyphs
\usepackage[english]{babel} % English language/hyphenation
\usepackage{amsmath,amsfonts,amsthm} % Math packages
\usepackage{mathrsfs}

\usepackage[margin=1in]{geometry}

\usepackage{sectsty} % Allows customizing section commands
\allsectionsfont{\centering \normalfont\scshape} % Make all sections centered, the default font and small caps

\usepackage{fancyhdr} % Custom headers and footers
\pagestyle{fancyplain} % Makes all pages in the document conform to the custom headers and footers
\fancyhead{} % No page header - if you want one, create it in the same way as the footers below
\fancyfoot[L]{} % Empty left footer
\fancyfoot[C]{} % Empty center footer
\fancyfoot[R]{\thepage} % Page numbering for right footer
\renewcommand{\headrulewidth}{0pt} % Remove header underlines
\renewcommand{\footrulewidth}{0pt} % Remove footer underlines
\setlength{\headheight}{13.6pt} % Customize the height of the header

\numberwithin{equation}{section} % Number equations within sections (i.e. 1.1, 1.2, 2.1, 2.2 instead of 1, 2, 3, 4)
\numberwithin{figure}{section} % Number figures within sections (i.e. 1.1, 1.2, 2.1, 2.2 instead of 1, 2, 3, 4)
\numberwithin{table}{section} % Number tables within sections (i.e. 1.1, 1.2, 2.1, 2.2 instead of 1, 2, 3, 4)

\newcommand{\R}{\mathbb{R}}
\newcommand{\Q}{\mathbb{Q}}
\newcommand{\N}{\mathbb{N}}
\newcommand{\C}{\mathbb{C}}

\newcommand{\tr}{\textrm{tr}}

\newtheorem{lemma}{Lemma}
%----------------------------------------------------------------------------------------
%	TITLE SECTION
%----------------------------------------------------------------------------------------

\newcommand{\horrule}[1]{\rule{\linewidth}{#1}} % Create horizontal rule command with 1 argument of height

\title{	
\normalfont \normalsize 
\textsc{Analysis} \\ [25pt] % Your university, school and/or department name(s)
\horrule{0.5pt} \\[0.4cm] % Thin top horizontal rule
\huge Homework 5 \\ % The assignment title
\horrule{2pt} \\[0.5cm] % Thick bottom horizontal rule
}

\author{Daniel Halmrast} % Your name

\date{\normalsize\today} % Today's date or a custom date

\begin{document}

\maketitle % Print the title

% Problems
\section*{Problem 1}
Let $E,F$ be closed subspaces of a Hilbert space. Prove that $P_EP_F=P_E$ if and
only if $E\subseteq F$.
\\
\\
\begin{proof}
    Suppose first that $P_EP_F=P_E$. Then, in particular,
    \[
        P_E^* = (P_EP_F)^* = P_F^*P_E^* = P_FP_E = P_E
    \]
    by self-adjointness of projections. Thus, $P_EP_F=P_FP_E=P_E$, and the
    projections commute. Thus, the von Neumann algebra $W^*(P_E,P_F,I)$ is
    Abelian, and is isometrically $*$-isomorphic to $L^{\infty}(X,\mu)$ for some
    measure space $(X,\mu)$. In particular, the projections $P_E,P_F$ get sent
    to self-adjoint idempotents $P_E\mapsto M_{\chi_S}$ and $P_F\mapsto
    M_{\chi_{S'}}$ for some measurable subsets $S,S'\subset X$.

    Now, the requirement $P_FP_E=P_E$ corresponds to the requirement
    \[
        M_{\chi_{S'}}M_{\chi_S}=M_{\chi_S}
    \]
    which means that $S\subset S'$. This, in turn, implies that $E\subset F$.

    Indeed, $E$ is the subspace of $H$ on which $P_E$ is the identity, which
    corresponds to the subspace
    \[
        \tilde{E} = \int_S^{\oplus}H(x)d\mu(x)
    \]
    on which $M_{\chi_S}$ is the identity. Similarly,
    \[
        \tilde{F} = \int_{S'}^{\oplus}H(x)d\mu(x)
    \]
    Clearly, $\tilde{E}\subset \tilde{F}$ (since $S\subset S'$) and so $E\subset
    F$ as well.
    \\
    \\
    For the converse direction, assume that $E\subset F$. Then, on $F$, $P_F =
    I_F$, and $P_FP_E = I_FP_E = P_E$. Furthermore, on $F^{\perp}$, $P_FP_E = 0
    = P_E$. Thus, on all of $H=F\oplus F^{\perp}$, $P_FP_E=P_E$ as desired.
\end{proof}

\newpage

\section*{Problem 2}
Characterize the closed subspaces $E,F$ of a Hilbert space $H$ satisfy
$P_FP_E=P_EP_F$.
\\
\\
\begin{proof}
    I assert that $P_E$ and $P_F$ commute if and only if $H$ can be decomposed
    into the four orthogonal components
    \[
        H = E\cap F\oplus E\cap F^{\perp}\oplus E^{\perp}\cap F\oplus
        E^{\perp}\cap F^{\perp}
    \]

    To see this, suppose first that $P_E$ and $P_F$ commute. Then, consider the
    Abelian von Neumann algebra $W^*(P_E,P_F,I)$. Like before, we use the Borel
    functional calculus to identify $W^*(P_E,P_F,I)$ with $L^{\infty}(X,\mu)$
    acting on $\tilde{H} = \int_X^{\oplus}H(x)d\mu(x)$, which is unitarily
    equivalent to $H$ (in the sense that there is a unitary transformation $U$
    such that $\tilde{H}=UH$ and $UW^*(P_E,P_F,I)U^*=L^{\infty}(X,\mu)$).

    Under this identification, $P_E\mapsto M_{\chi_S}$, and $P_F\mapsto
    M_{\chi_{S'}}$ for some measurable subsets $S,S'\subset X$. In particular,
    this decomposes $\tilde{H}$ into four orthogonal components
    \[
        \begin{aligned}
            \tilde{H} &= \int_X^{\oplus}H(x)d\mu(x)\\
            &= \int_{S\cap S'}^{\oplus}H(x)d\mu(x)\oplus 
            \int_{S\cap S'^c}^{\oplus}H(x)d\mu(x)\oplus
            \int_{S'\cap S^c}^{\oplus}H(x)d\mu(x)\oplus
            \int_{S^c\cap S'^c}^{\oplus}H(x)d\mu(x)
        \end{aligned}
    \]
    which translates into the decomposition on $H$ as
    \[
        H = E\cap F\oplus E\cap F^{\perp}\oplus E^{\perp}\cap F\oplus
        E^{\perp}\cap F^{\perp}
    \]
    as desired.
    \\
    \\
    Conversely, suppose $H$ can be decomposed this way. Then, let $v\in H$ be
    decomposed as 
    \[
        v= v_1 + v_2 + v_3 + v_4
    \]
    where $v_1\in E\cap F$, $v_2\in E\cap F^{\perp}$, $v_3\in E^{\perp}\cap F$
    and $v_4\in E^{\perp}\cap F^{\perp}$.

    We compute the effect of $P_EP_F$ and $P_FP_E$ directly.
    \[
\begin{aligned}
    P_EP_F(v) &= P_EP_F(v_1+v_2+v_3+v_4)\\
    &= P_E(v_1 + v_3)\\
    &= v_1\\
    P_FP_E(v) &= P_FP_E(v_1+v_2+v_3+v_4)\\
    &=P_F(v_1+v_2)\\
    &=v_1
\end{aligned}
    \]
    and thus $P_EP_F=P_FP_E$ as desired.
\end{proof}

\newpage

\section*{Problem 3}
Let $E,F$ be closed subspaces of a Hilbert space $H$. An operator $U$ is said to
be a partial isometry from $E$ to $F$ if $U|_E$ is an isometry onto $F$, and
$U|_{E^{\perp}}=0$.
Prove that $U$ is a partial isometry $\iff$ $U^*U$ is a projection $\iff$ $UU^*$
is a projection.
\\
\\
\begin{proof}
    Suppose first that $U$ is a partial isometry from $E$ to $F$. I assert that
    $U^*U = P_E$. To see this, suppose $e\in E$, $v\in H$ and let $v=e'+v'$
    where $e'\in E$ and $v'\in E^{\perp}$. Then,
    \[
        \begin{aligned}
            \langle U^*Ue|v\rangle &= \langle U^*Ue|e'+v'\rangle\\
            &= \langle Ue|Ue'\rangle + \langle Ue|Uv'\rangle\\
            &= \langle e|e'\rangle + 0\\
            \implies \langle U^*Ue-e|v\rangle&=0
        \end{aligned}
    \]
    and since this holds for all $v\in H$, $U^*Ue-e=0$ and thus $U^*Ue=e$ and
    $U^*U$ is the identity on $E$.

    Furthermore, for $v'\in E^{\perp}$,
    \[
        U^*Uv'=U^*(0) = 0
    \]
    and so $U^*U$ is the zero map on $E^{\perp}$. Thus, $U^*U$ agrees with $P_E$
    at all points, so $U^*U=P_E$ as desired.
    \\
    \\
    Conversely, suppose $U^*U$ is a projection $P_E$ for some closed subspace
    $E$. Define $F=U(E)$. We will first show that $U$ is an isometry of $E$ onto
    $F$. To see this, suppose $e,e'\in E$. We calculate directly
    \[
\begin{aligned}
    \langle Ue|Ue'\rangle &= \langle U^*Ue|e'\rangle\\
    &=\langle P_Ee|e'\rangle\\
    &=\langle e|e'\rangle
\end{aligned}
    \]
    and thus $U$ is an isometry from $E$ to $F$. Note that this immediately
    implies that $F$ is a closed subspace. Finally, we show that
    $U|_{E^{\perp}}=0$. Let $v'\in E^{\perp}$, Then,
    \[
\begin{aligned}
    \|Uv'\| &=\langle Uv'|Uv'\rangle\\
    &=\langle U^*Uv'|v'\rangle\\
    &=\langle 0|v'\rangle = 0
\end{aligned}
    \]
    and so $U^*U|_{E^{\perp}}=0$ as desired. Thus, $U$ is a partial isometry.
    \\
    \\
    Finally, we show that if $U$ is a partial isometry, then $U^*$ is a partial
    isometry, which will complete the proof. So, suppose $U$ is a partial
    isometry. We will show that $U^*$ is a partial isometry from $F$ to $E$.
    First, we check that $U^*|_F$ is an isometry. Now, for each $f\in F$, there
    is some $e\in E$ with $Ue=f$. Thus, for $e,e'\in E$, $f,f'\in F$ with
    $Ue=f,Ue'=f'$,
    \[
        \begin{aligned}
            \langle U^*f|U^*f'\rangle &= \langle U^*Ue|U^*Ue\rangle\\
            &=\langle P_Ee|P_Ee'\rangle\\
            &=\langle e|e'\rangle\\
            &=\langle Ue|Ue'\rangle\\
            &=\langle f|f'\rangle
        \end{aligned}
    \]
    and so $U^*$ is an isometry from $F$ to $E$.
    Finally, we show that $U^*|_{F^{\perp}}=0$. This is immediate, since
    \[
        \begin{aligned}
            \ker U^* = U(H)^{\perp} = F^{\perp}
        \end{aligned}
    \]
    where we used the identity $\ker A^* = A(H)^{\perp}$ for all bounded
    operators $A$. 

    Note that this completes the proof. If $U$ is a partial isometry, then $U^*$
    is a partial isometry, which implies that $U^{**}U^*=UU^*$ is a projection.
    Similarly, if $UU^*=U^{**}U^*$ is a projection, then $U^*$ is a partial
    isometry, and thus $U^{**}=U$ is a partial isometry as well.
\end{proof}

\newpage

\section*{Problem 4}
Prove that the subspace of self-adjoint operators on $B(\C^2)$ is a subset of
the linear subspace spanned (over $\R$) by $I$ and the three Pauli matrices
\[
\sigma_1 =
\begin{bmatrix}
    1&0\\
    0&-1
\end{bmatrix}
,\ 
\sigma_2 = 
\begin{bmatrix}
    0&1\\
    1&0
\end{bmatrix}
,\ 
\sigma_3 = 
\begin{bmatrix}
    0&i\\
    -i&0
\end{bmatrix}
\]

and prove that the span of $\{\sigma_i\}_{i=1}^3$ is isometrically isomorphic to
a three-dimensional real Hilbert space under the operator norm.
\\
\\
\begin{proof}
    We observe first that for any $T\in B(\C^2)$ self-adjoint, we have the
    condition
    \[
        T^i_j = \overline{T^j_i}
    \]
    In particular,
    \[
        \begin{aligned}
            T^1_1 = \overline{T^1_1}\\
            T^2_2 = \overline{T^2_2}\\
        \end{aligned}
    \]
    and so $T^i_i$ is real. Furthermore, we have the relation
    \[
        T^1_2 = \overline{T^2_1}
    \]
    Finally, we observe that we can decompose $T$ into a scalar part and a
    trace-free part by
    \[
\begin{aligned}
    C = T-\tr(T)I\\
    T = \tr(T)I + C\\
\end{aligned}
    \]

    Now we are ready to show that $T$ is a linear combination of $I$ and the
    Pauli matrices. In particular, we will show that $C$ is a linear combination
    of the Pauli matrices.

    For $C$, we have the relations
    \[
        \begin{aligned}
        C^1_1 = -C^2_2\\
        C^1_2 = \overline{C^2_1}
    \end{aligned}
    \]
    as well as the requirement that $C^1_1$ is real. Thus, we have three degrees
    of freedom. That is,
    \[
        C = 
        \begin{bmatrix}
            \alpha &\beta+\gamma i\\
            \beta-\gamma i&-\alpha
        \end{bmatrix}
    \]
    which decomposes as
    \[
        C = \alpha\sigma_1 + \beta\sigma_2 +\gamma\sigma_3
    \]
    and so
    \[
        T = \tr(T)I + C
    \]
    is a linear combination of $I$ and $\{\sigma_i\}_{i=1}^3$ as desired.
    \\
    \\
    Next, we show that the span of $\{\sigma_i\}_{i=1}^3$ under the operator
    norm is isometrically isomorphic to $\R^3$. To do so, we will show that the
    operator norm coincides with the pullback metric from $\R^3$. Specifically,
    we define a linear isomorphism
    \[
        \begin{aligned}
        \Phi:\langle \sigma_i\rangle_{i=1}^3\to \R^3\\
        \Phi(\sigma_i) = e_i
    \end{aligned}
    \]
    where $\{e_i\}$ is an orthonormal basis for $\R^3$ with its usual inner
    product. In particular, if we denote the inner product of $\R^3$ as $\eta$,
    we can define $\Phi^*(\eta)$ by
    \[
        \Phi^*(\eta)(u,v) = \eta(\Phi(u),\Phi(v))
    \]
    In order to show that this metric coincides with the operator norm, we have
    to show that
    \[
        \|\alpha\sigma_1+\beta\sigma_2+\gamma\sigma_3\|^2 =
        \Phi^*(\eta)(\alpha\sigma_1+\beta\sigma_2+\gamma\sigma_3,
        \alpha\sigma_1+\beta\sigma_2+\gamma\sigma_3) = \alpha^2+\beta^2+\gamma^2
    \]
    Now, since $\sigma_i$ are all self-adjoint, any (real) linear combination of
    them will be as well. Thus,
    \[
    \|\alpha\sigma_1+\beta\sigma_2+\gamma\sigma_3\|^2 =
\|(\alpha\sigma_1+\beta\sigma_2+\gamma\sigma_3)^2\|
    \]
    We compute the right-hand side directly
    \[
\begin{aligned}
    (\alpha\sigma_1+\beta\sigma_2+\gamma\sigma_3)^2 &=
    \alpha^2\sigma_1^2 + \beta^2\sigma_2^2  + \gamma\sigma_3^2 +
    \alpha\beta\{\sigma_1,\sigma_2\} + \alpha\gamma\{\sigma_1,\sigma_3\} +
    \beta\gamma\{\sigma_2,\sigma_3\}
\end{aligned}
    \]
    where $\{\sigma_i,\sigma_j\}$ is the anticommutator of $\sigma_i$ and
    $\sigma_j$. Now, it is well-known that the Pauli matrices satisfy the
    commutation relations
    \[
        [\sigma_i,\sigma_j]=2i\varepsilon_{ijk}\sigma_k
    \]
    as well as the relation
    \[
        \sigma_i^2 = I
    \]
    (where $\varepsilon_{ijk}$ is the levi-civita symbol) which forces
    \[
        \sigma_i\sigma_j = i\varepsilon_{ijk}\sigma_k + \delta_{ij}
    \]
    and so
    \[
        \begin{aligned}
        \{\sigma_i,\sigma_j\} &= \sigma_i\sigma_j + \sigma_j\sigma_i\\
        &= i\varepsilon_{ijk}\sigma_k + \delta_{ij} + i\varepsilon_{jik}\sigma_k +
        \delta_{ji}\\
        &= i\varepsilon_{ijk}\sigma_k - i\varepsilon_{ijk}\sigma_k +
        2\delta_{ij}\\
        &= 2\delta_{ij}
    \end{aligned}
    \]

    Thus,
    \[
\begin{aligned}
    (\alpha\sigma_1+\beta\sigma_2+\gamma\sigma_3)^2 &=
    \alpha^2\sigma_1^2 + \beta^2\sigma_2^2  + \gamma\sigma_3^2 +
    \alpha\beta\{\sigma_1,\sigma_2\} + \alpha\gamma\{\sigma_1,\sigma_3\} +
    \beta\gamma\{\sigma_2,\sigma_3\}\\
    &= 
    \alpha^2\sigma_1^2 + \beta^2\sigma_2^2  + \gamma\sigma_3^2\\
    &=(\alpha^2+\beta^2+\gamma^2)I
\end{aligned}
    \]
    and so
    \[
    \|\alpha\sigma_1 + \beta^2\sigma_2 + \gamma\sigma_3\|^2 =
    \|(\alpha^2+\beta^2+\gamma^2)I\| = (\alpha^2+\beta^2+\gamma^2)\|I\|
    =(\alpha^2+\beta^2+\gamma^2)
    \]
    as desired. Thus, the pullback metric coincides with the operator norm, and
    $\Phi$ is a linear isometric isomorphism, as desired.
\end{proof}

\newpage

\section*{Problem 5}
Let $H$ be a separable Hilbert space. Prove $T^*T$ is positive for all $T\in
B(H)$. Prove that every positive operator is equal to $T^*T$ for some $T\in
B(H)$. Can we ensure $T$ is self-adjoint?
\\
\\
\begin{proof}
    First, we show $T^*T$ is positive. That is, we need to show that
    \[
\langle T^*T\eta|\eta\rangle\geq 0\forall \eta\in H
    \]
    This follows immediately, since
    \[
        \begin{aligned}
            \langle T^*T\eta|\eta\rangle &= \langle T\eta|T\eta\rangle\\
            &= \|T\eta\|^2 \geq 0
        \end{aligned}
    \]
    and thus $T^*T$ is positive.
    \\
    \\
    Next, we show that every positive operator can be written this way. In
    particular, let $A$ be a positive operator. We know that $\sigma(A)\subset
    [0,\infty)$, since $A$ is positive. Therefore, the square root function is
    defined on $\sigma(A)$. Through the continuous functional calculus, we can
    define
    \[
        \sqrt{A} = \int_{\sigma(A)}\sqrt{z}dE(z)
    \]
    for $E$ the projection-valued measure associated to $A$ (so that $A
    =\int_{\sigma(A)}zdE(z)$). This satisfies
    \[
        \begin{aligned}
        \sqrt{A}\sqrt{A} &=
        \int_{\sigma(A)}\sqrt{z}dE(z)\int_{\sigma(A)}\sqrt{z}dE(z)\\
        &= \int_{\sigma(A)}\sqrt{z}\sqrt{z}dE(z)\\
        &=\int_{\sigma(A)}zdE(z) = A
    \end{aligned}
    \]
    and so by setting $T=T^*=\sqrt{A}$ we achieve the desired result.
\end{proof}

\newpage

\section*{Problem 6}
Let $H$ be a separable Hilbert space, and let $T\in B(H)$ be self-adjoint.
Suppose $\sigma(T) = [-\varepsilon,\varepsilon]\cup
[1-\varepsilon,1+\varepsilon]$. Prove there is a projection $P$ for which
$\|T-P\|\leq \varepsilon$.
\\
\\
\begin{proof}
    Let $E$ be the projection-valued measure associated to $T$, so that
    \[
\begin{aligned}
    T &= \int_{\sigma(T)}zdE(z)\\
    I &= \int_{\sigma(T)}dE(z)
\end{aligned}
    \]
    and define
    \[
        P = \int_{\sigma(T)}\chi_{[1-\varepsilon,1+\varepsilon]}(z)dE(z)
        = E([1-\varepsilon,1+\varepsilon])
    \]
    which is a projection. Then,
    \[
        \begin{aligned}
            T-P &=
            \int_{\sigma(T)}(z-\chi_{[1-\varepsilon,1+\varepsilon]}(z))dE(z)\\
        \end{aligned}
    \]
    Let $f=z-\chi_{[1-\varepsilon,1+\varepsilon]}(z)$, defined on $\sigma(T)$.
    Now, $\|f\|_{\infty} = \varepsilon$, and so
    \[
        \begin{aligned}
        \|T-P\|^2 &= \sup_{h\in H,\|h\|=1}\langle \int fdE h|\int fdE h\rangle\\
        &=\sup_{h\in H,\|h\|=1}\langle\int \bar{f}dE\int fdE h|h\rangle\\
        &=\sup_{h\in H,\|h\|=1}\langle \int |f|^2dE h|h\rangle\\
        &=\sup_{h\in H,\|h\|=1}\int |f|^2d\mu_{h,h}\\
        &\leq \sup_{h\in H,\|h\|=1}\||f|^2\|_{\infty}\int d\mu_{h,h}\\
        &\leq \sup_{h\in H,\|h\|=1}\||f|\|^2_{\infty}\int d\mu_{h,h}\\
        &= \sup_{h\in H,\|h\|=1}\||f|\|^2_{\infty}\|h\|^2 = \||f|\|^2_{\infty}
    \end{aligned}
    \]
    where $\mu_{h,g}$ is the induced (complex) measure defined as
    \[
        \mu_{h,g}(S) = \langle E(S)h|g\rangle
    \]
    Thus,
    \[
        \|T-P\|\leq \|f\|_{\infty} = \varepsilon
    \]
    as desired.
\end{proof}

\newpage

\section*{Problem 7}
Let $H$ be a separable complex Hilbert space, $T\in B(H)$ self-adjoint, and
suppose $T$ is invertible. Find a continuous path (with respect to the norm
topology) from $T$ to $I$ that stays in $GL(H)\subset B(H)$ the invertible
elements of $B(H)$. Can we also ensure the path stays in the self-adjoint subset
of $GL(H)$?
\\
\\
\begin{proof}
    Recall that every operator $T\in B(H)$, $T$ has a polar decomposition
    \[
        T=PU
    \]
    where $P$ is positive and $U$ is a partial isometry. Furthermore, if $T$ is
    invertible, then $U$ is unitary. So, let $T$ be decomposed as such.
    Furthermore, we write
    \[
        \begin{aligned}
            P=\exp(Q)\\
            U=\exp(iH)
        \end{aligned}
    \]
    for self-adjoint $Q$ and $H$ ($Q$ is just $\log(P)$, and $H$ is guaranteed
    to exist for unitary operators as the generator for $U$).

    Now, we can write
    \[
        T = \exp(Q+iH)
    \]
    and define a one-parameter group of operators
    \[
        T_t = \exp(t(Q+iH))
    \]
    with the property that $T_0 = I$, $T_1=T$, and $T_tT_{-t}=I$ for all $t$.
    Thus, this one-parameter group is a subset of $GL(H)$, and has endpoints at
    $I$ and $T$, as desired. Furthermore, it is continuous in $T$, since
    \[
        T_t = \exp(tQ)\exp(tiH)
    \]
    and $\exp(tQ),\exp(tiH)$ are both continuous with respect to $t$, so their
    product is as well.

    Now, we cannot guarantee that any path will stay in the self-adjoint subset
    of $GL(H)$. Take for a counterexample $B(H)=H=\C$, $T=-1$. The self-adjoint
    invertible operators in $\C$ are $\R\setminus\{0\}$, which has two path
    components. $-1$ and $1$ are not in the same path-component, so there cannot
    be a path that joins them in the self-adjoint subset of $\C$.
\end{proof}

\newpage

\section*{Problem 8}
Let $H$ be a separable Hilbert space, and $\mathscr{A}\subset B(H)$ a $C^*$
algebra containing $T$ a self-adjoint invertible operator. Prove that $T^{-1}$
lies in $\mathscr{A}$.
\\
\\
\begin{proof}
    Recall that $C^*(T)$ is the minimal unital $C^*$ algebra containing $T$.
    In particular, $C^*(T)\subset \mathscr{A}$. So, we will show that
    $T^{-1}\in\mathscr{A}$.

    Recall that the continuous functional calculus gives us a isometric
    $*$-isomorphism (say, $\gamma$) between $C^*(T)$ and $C(\sigma(T))$ in the
    sup norm. In particular, since $T$ is invertible, $0\not\in\sigma(T)$, and
    so the function $f(z) = z^{-1}$ is well-defined. Furthermore, we know that
    \[
        \gamma(T)=z
    \]
    and so
    \[
\begin{aligned}
    I &= \gamma^{-1}(1)\\
    &= \gamma^{-1}(zz^{-1})\\
    &= \gamma^{-1}(z)\gamma^{-1}(z^{-1})\\
    &= T\gamma^{-1}(z^{-1})
\end{aligned}
    \]
    and thus $\gamma^{-1}(z^{-1})$ is the inverse of $T$, as desired. Thus,
    $T^{-1}$ is in $C^*(T)\subset\mathscr{A}$, as desired.
\end{proof}

\end{document}
